lib_misc/SteelVRefineDep.fsti
@@ -1,0 +1,118 @@
+module SteelVRefineDep
+
+open Steel.Effect.Atomic
+open Steel.Effect
+
+module SM = Steel.Memory
+module G = FStar.Ghost
+
+val vrefinedep_hp
+  (v: vprop)
+  (p: ( (t_of v) -> Tot prop))
+  (f: ( t_of (vrefine v p) -> Tot vprop))
+  : Tot (SM.slprop u#1)
+
+[@__steel_reduce__]
+let vrefinedep_t
+  (v: vprop)
+  (p: ( (t_of v) -> Tot prop))
+  (f: ( t_of (vrefine v p) -> Tot vprop))
+  : Tot Type
+  =
+  dtuple2 (t_of (vrefine v p)) (fun x -> t_of (f x))
+
+val vrefinedep_sel
+  (v: vprop)
+  (p: ( (t_of v) -> Tot prop))
+  (f: ( (t_of (vrefine v p)) -> Tot vprop))
+  : Tot (selector (vrefinedep_t v p f) (vrefinedep_hp v p f))
+
+[@@__steel_reduce__]
+let vrefinedep'
+  (v: vprop)
+  (p: ( (t_of v) -> Tot prop))
+  (f: ( (t_of (vrefine v p)) -> Tot vprop))
+  : Tot vprop' = {
+  hp = vrefinedep_hp v p f;
+  t = vrefinedep_t v p f;
+  sel = vrefinedep_sel v p f;
+}
+[@@__steel_reduce__]
+let vrefinedep
+  (v: vprop)
+  (p: ( (t_of v) -> Tot prop))
+  (f: ( (t_of (vrefine v p)) -> Tot vprop))
+  = VUnit (vrefinedep' v p f)
+
+val elim_vrefinedep
+  (#opened:_)
+  (v: vprop)
+  (p: ( (t_of v) -> Tot prop))
+  (f: ( (t_of (vrefine v p)) -> Tot vprop))
+  : SteelGhost (G.erased (t_of (vrefine v p))) opened
+  (vrefinedep v p f)
+  (fun res -> v `star` f (G.reveal res))
+  (requires fun _ -> True)
+  (ensures fun h res h' ->
+    let (res : normal (t_of v){p res}) = res in
+    p res /\
+    G.reveal res == h' v /\
+    (let fs : x:t_of v{p x} = h' v in
+    let sn : t_of (f (G.reveal res)) = h' (f (G.reveal res)) in
+    let x2 = h (vrefinedep v p f) in
+    G.reveal res == fs /\
+    dfst x2 == fs /\
+    dsnd x2 == sn /\
+    True)
+  )
+
+val intro_vrefinedep
+  (#opened:_)
+  (v: vprop)
+  (p: ( (t_of v) -> Tot prop))
+  (f: ( (t_of (vrefine v p)) -> Tot vprop))
+  (f': vprop)
+  : SteelGhost unit opened
+  (v `star` f')
+  (fun _ -> vrefinedep v p f)
+  (requires fun h ->
+    p (h v) /\
+    f' == f (h v))
+  (ensures fun h _ h' ->
+    p (h v) /\
+    f' == f (h v) /\
+    (let x2 = h' (vrefinedep v p f) in
+    let sn : t_of f' = h f' in
+    dfst x2 == h v /\
+    dsnd x2 == sn)
+  )
+
+#push-options "--compat_pre_typed_indexed_effects"
+#push-options "--z3rlimit 20"
+let vrefinedep_idem
+  (#opened:_)
+  (v: vprop)
+  (p: ( (t_of v) -> Tot prop))
+  (f: ( (t_of (vrefine v p)) -> Tot vprop))
+  : SteelGhost unit opened
+  (vrefinedep v p f)
+  (fun _ -> vrefinedep v p f)
+  (requires fun _ -> True)
+  (ensures fun h _ h' ->
+    h (vrefinedep v p f)
+    ==
+    h' (vrefinedep v p f)
+  )
+  =
+  //let h0 = get () in
+  let x0 = gget (vrefinedep v p f) in
+  let x = elim_vrefinedep v p f in
+  intro_vrefinedep v p  f (f (G.reveal x));
+  //let h1 = get () in
+  let x1 = gget (vrefinedep v p f) in
+  assert (dfst x0 == dfst x1);
+  assert (dsnd x0 == dsnd x1);
+  //assert (x0 == x1);
+  ()
+#pop-options
+#pop-options
